src/tls/StreamAE.fst
@@ -153,7 +153,7 @@ val genReader: parent:rid -> #i:id -> w:writer i -> ST (reader i)
 
 let genReader parent #i w =
   let reader_r = new_region parent in
-  let raead = AEAD.genReader w.aead in
+  let raead = AEAD.genReader parent w.aead in
   if authId i then
     let log : ideal_log w.region i = w.log in
     let dctr: ideal_ctr reader_r i log = new_seqn reader_r 0 log in
@@ -211,7 +211,7 @@ let encrypt #i e l p =
   let n = m_read ctr in
   let nb = bytes_of_int (AEAD.noncelen i) n in
   let iv = AEAD.create_nonce e.aead nb in
-  let c = AEAD.encrypt i e.aead iv noAD text in
+  let c = AEAD.encrypt #i #l e.aead iv noAD text in
   if authId i then
     begin
     let ilog = ilog e.log in
@@ -274,7 +274,7 @@ let decrypt #i d l c =
   else //concrete
    let nb = bytes_of_int (AEAD.noncelen i) j in
    let iv = AEAD.create_nonce d.aead nb in
-   match AEAD.decrypt i d.aead iv noAD c with
+   match AEAD.decrypt #i #l d.aead iv noAD c with
    | None -> None
    | Some pr ->
      begin
